backends/lean/Aeneas/Tactic/Step/Step.lean
@@ -176,6 +176,12 @@ structure Stats extends Goals where
 attribute [step_post_simps]
   Std.IScalar.toNat Std.UScalar.ofNatCore_toNat_eq Std.IScalar.ofInt_toInt_eq
 
+open Std ScalarElab in
+uscalar attribute [step_post_simps] «%S».ofNatCore_toNat_eq
+
+open Std ScalarElab in
+iscalar attribute [step_post_simps] «%S».toNat «%S».ofInt_toInt_eq
+
 structure Args where
   /-- Asynchronously solve the preconditions? **DO NOT USE**: this is experimental and triggers bugs -/
   async : Bool
